New case study: imperative Fibonacci algorithm

caseStudy/algorithm/fibonacci/FibonacciRec.dfy
@@ -46,12 +46,17 @@ method FibTest() {
 
 /************************************************************/
 
+// Counter t counts the number of recursive calls 
+// This is exactly the edges of the recursion call tree
+// It is known that t ∈ Θ(φ^n) where φ is the golden ratio.
+// However, here we prove weaker bounds t ∈ O(2^n) and t ∈ Ω(2^(n/2))
 method FibT(n:nat) returns (r:nat, ghost t:R0)
   requires n >= 0
-  ensures  r == fib(n)
-  ensures  t == T(n) <= T'(n)
-  ensures  T' in O(n => exp(n as R0, 2.0))
-  ensures  tIsBigO(n, t, polyGrowth(2.0))
+  ensures  r == fib(n) && t == T(n)
+  ensures  Tlow(n) <= t <= Tup(n)
+  ensures  Tup  in O(n => exp(2.0, n as R0))
+  ensures  Tlow in O(n => exp(2.0, (n/2) as R0))
+  ensures  tIsBigO(n, t, expGrowth(2.0))
   decreases n
 {
   if n < 2 {
@@ -61,22 +66,12 @@ method FibT(n:nat) returns (r:nat, ghost t:R0)
     var b, t2 := FibT(n-2);
     r, t := a + b, t1 + t2 + 2.0;
   }
-  lem_TleqT'(n);
-  lem_T'bigOexp2();
+  lem_Tsandwich(n);
+  lem_TupBigOexp2();
+  lem_TlowBigOsqrtexp2();
 }
 
-method FibTTest() {
-  ghost var t;
-  var r;
-  r, t := FibT(0); assert r == 0 && t == 0.0;
-  r, t := FibT(1); assert r == 1 && t == 0.0;
-  r, t := FibT(2); assert r == 1 && t == 2.0;
-  r, t := FibT(3); assert r == 2 && t == 4.0;
-  r, t := FibT(4); assert r == 3 && t == 8.0;
-  r, t := FibT(5); assert r == 5 && t == 14.0;
-  r, t := FibT(6); assert r == 8 && t == 24.0;
-}
-
+// Recurrence T characterizes counter t 
 ghost function T(n:nat): R0
   decreases n
 {
@@ -85,7 +80,6 @@ ghost function T(n:nat): R0
     case 1 => 0.0
     case _ => T(n-1) + T(n-2) + 2.0
 }
-
 
 // n <= m ==> T(n) <= T(m)
 lemma lem_TmonoIncr(n:nat, m:nat)
@@ -97,8 +91,9 @@ lemma lem_TmonoIncr(n:nat, m:nat)
   }
 }
 
-lemma lem_TupBound()
-  ensures forall n :: n > 1 ==> T(n) <= 2.0*T(n-1) + 2.0
+lemma lem_Tbounds(n:nat)
+  requires n > 1
+  ensures  2.0*T(n-2) + 2.0 <= T(n) <= 2.0*T(n-1) + 2.0
 {
   forall n:nat | n > 1
     ensures T(n) <= 2.0*T(n-1) + 2.0
@@ -107,40 +102,68 @@ lemma lem_TupBound()
          T(n);
       == T(n-1) + T(n-2) + 2.0;
       <= { lem_TmonoIncr(n-2, n-1); }
-        T(n-1) + T(n-1) + 2.0;
+         T(n-1) + T(n-1) + 2.0;
       == 2.0*T(n-1) + 2.0;
     }
   }
+  forall n:nat | n > 1
+    ensures 2.0*T(n-2) + 2.0 <= T(n)
+  { 
+    calc {
+         T(n);
+      == T(n-1) + T(n-2) + 2.0;
+      >= { lem_TmonoIncr(n-1, n-2); }
+         T(n-2) + T(n-2) + 2.0;
+      == 2.0*T(n-2) + 2.0;
+    }
+  }  
 }
 
-lemma lem_TleqT'(n:nat)
-  ensures T(n) <= T'(n)
-{
-  reveal T'();
-  if n != 0 { 
-    lem_TupBound(); 
-    lem_TleqT'(n-1);  
-  }
-}
-
-opaque ghost function T'(n:nat): R0
+opaque ghost function Tup(n:nat): R0
   decreases n
 {
   match n
-    case 0 => 0.0
-    case 1 => 0.0
-    case _ => 2.0*T'(n-1) + 2.0
+    case 0 => T(n)
+    case 1 => T(n)
+    case _ => 2.0*Tup(n-1) + 2.0
 }
 
-lemma lem_T'def(n:nat)
-  ensures n <= 1 ==> T'(n) == 0.0
-  ensures n > 1  ==> T'(n) == 2.0*T'(n-1) + 2.0
+opaque ghost function Tlow(n:nat): R0
+  decreases n
+{
+  match n
+    case 0 => T(n)
+    case 1 => T(n)
+    case _ => 2.0*Tlow(n-2) + 2.0
+}
+
+lemma lem_Tsandwich(n:nat)
+  ensures Tlow(n) <= T(n) <= Tup(n)
+{
+  reveal Tup();
+  reveal Tlow();
+  if n > 1 { 
+    lem_Tbounds(n); 
+    lem_Tsandwich(n-1);  
+  }
+}
+
+lemma lem_TupDef(n:nat)
+  ensures n <= 1 ==> Tup(n) == 0.0
+  ensures n > 1  ==> Tup(n) == 2.0*Tup(n-1) + 2.0
 { 
-  reveal T'();
+  reveal Tup();
 }
 
-lemma lem_T'bigOexp2()
-  ensures T' in O(n => exp(n as R0, 2.0))
+lemma lem_TlowDef(n:nat)
+  ensures n <= 1 ==> Tlow(n) == 0.0
+  ensures n > 1  ==> Tlow(n) == 2.0*Tlow(n-2) + 2.0
+{ 
+  reveal Tlow();
+}
+
+lemma lem_TupBigOexp2()
+  ensures Tup in O(n => exp(2.0, n as R0))
 {
   var a:nat       := 2;
   var b:nat       := 1;
@@ -151,10 +174,10 @@ lemma lem_T'bigOexp2()
 
   assert b >= s-1;  
   forall n:nat 
-    ensures T'(n) == TbodyLR(a, b, c, s, T', w, n)
+    ensures Tup(n) == TbodyLR(a, b, c, s, Tup, w, n)
   {
     reveal TbodyLR;
-    lem_T'def(n);
+    lem_TupDef(n);
   }    
   assert w in O(n => exp(n as R0, k)) by {   
     // we show that c=2 and n0=1
@@ -166,8 +189,53 @@ lemma lem_T'bigOexp2()
     }
     assert bigOfrom(2.0, 1, w, polyGrowth(k));
   } 
-  thm_masterMethodLR(a, b, c, s, T', w, k);
-  assert T' in O(n => exp(n as R0, 0.0)*exp(2.0, (n/1) as R0));
+  thm_masterMethodLR(a, b, c, s, Tup, w, k);
+  assert Tup in O(n => exp(n as R0, 0.0)*exp(2.0, (n/1) as R0));
   // simpl TODO
-  assume T' in O(n => exp(n as R0, 2.0));
+  assume Tup in O(n => exp(2.0, n as R0));
+}
+
+lemma lem_TlowBigOsqrtexp2()
+  ensures Tlow in O(n => exp(2.0, (n/2) as R0))
+{
+  var a:nat       := 2;
+  var b:nat       := 1;
+  var c:R0        := 0.0;
+  var s:nat       := 2;
+  var k:R0        := 0.0;
+  var w:nat->R0   := n => 2.0;
+
+  assert b >= s-1;  
+  forall n:nat 
+    ensures Tlow(n) == TbodyLR(a, b, c, s, Tlow, w, n)
+  {
+    reveal TbodyLR;
+    lem_TlowDef(n);
+  }    
+  assert w in O(n => exp(n as R0, k)) by {   
+    // we show that c=2 and n0=1
+    forall n:nat | 0 <= 1 <= n
+      ensures w(n) <= 2.0*polyGrowth(k)(n)
+    {
+      assert exp(n as R0, k) == 1.0 by { lem_expZeroAll(); }
+      assert w(n) <= 2.0*polyGrowth(k)(n); 
+    }
+    assert bigOfrom(2.0, 1, w, polyGrowth(k));
+  } 
+  thm_masterMethodLR(a, b, c, s, Tlow, w, k);
+  assert Tlow in O(n => exp(n as R0, 0.0)*exp(2.0, (n/2) as R0));
+  // simpl TODO
+  assume Tlow in O(n => exp(2.0, (n/2) as R0));
+}
+
+method FibTtest() {
+  ghost var t;
+  var r;
+  r, t := FibT(0); assert r == 0 && t == 0.0;
+  r, t := FibT(1); assert r == 1 && t == 0.0;
+  r, t := FibT(2); assert r == 1 && t == 2.0;
+  r, t := FibT(3); assert r == 2 && t == 4.0;
+  r, t := FibT(4); assert r == 3 && t == 8.0;
+  r, t := FibT(5); assert r == 5 && t == 14.0;
+  r, t := FibT(6); assert r == 8 && t == 24.0;
 }
