caseStudy/algorithm/fibonacci/FibonacciImp.dfy
@@ -1,0 +1,129 @@
+include "../../../theory/math/ExpReal.dfy"
+include "../../../theory/math/SumReal.dfy"
+include "../../../theory/math/TypeR0.dfy"
+include "../../../theory/ComplexityR0.dfy"
+include "../../../theory/MasterLR.dfy"
+
+import opened ExpReal
+import opened SumReal
+import opened TypeR0
+import opened ComplexityR0
+import opened MasterLR
+
+ghost function fib(n:nat): nat
+  decreases n
+{
+  match n
+    case 0 => 0
+    case 1 => 1
+    case _ => fib(n-1) + fib(n-2)
+}
+
+method Fib(n:nat) returns (r:nat)
+  requires n >= 0
+  ensures  r == fib(n)
+{
+  var i, f1, f2 := 0, 0, 1;
+  while (i < n)
+    invariant 0 <= i <= n
+    invariant f1 == fib(i)
+    invariant f2 == fib(i+1)
+  {
+    var tmp := f1 + f2;
+    f1 := f2;
+    f2 := tmp;
+    i := i + 1;
+  }
+  r := f1;
+}
+
+method FibTest() {
+  var r;
+  r := Fib(0); assert r == 0;
+  r := Fib(1); assert r == 1;
+  r := Fib(2); assert r == 1;
+  r := Fib(3); assert r == 2;
+  r := Fib(4); assert r == 3;
+  r := Fib(5); assert r == 5;
+  r := Fib(6); assert r == 8;
+}
+
+/************************************************************/
+
+ghost function f(n:nat) : R0
+{ 
+  n as R0 
+}
+
+method FibT(n:nat) returns (r:nat, ghost t:R0)
+  requires n >= 0
+  ensures  r == fib(n)
+  ensures  t == f(n)
+  ensures  tIsBigO(n, t, linGrowth())
+{
+  t := 0.0; reveal T();
+  var i, f1, f2 := 0, 0, 1;
+  while i < n
+    invariant 0 <= i <= n
+    invariant f1 == fib(i)
+    invariant f2 == fib(i+1)
+    invariant t == T(i)              // = T(n)- T(i)
+    invariant t == T2(n,0) - T2(n,i) // = T2(i)
+    invariant t == i as R0
+    decreases n - i
+  {
+    var tmp := f1 + f2;
+    f1 := f2;
+    f2 := tmp;
+    i := i + 1;
+    t := t + 1.0;
+  }
+  r := f1;
+  assert t == n as R0; 
+  assert f in O(linGrowth()) by { var c, n0 := lem_fBigOlin(); }
+}
+
+ghost function T(n:nat): R0
+  decreases n
+{
+  if n == 0 then 0.0 else T(n-1) + 1.0
+}
+
+ghost function T2(N:nat, i:nat): R0
+  requires 0 <= i <= N
+  decreases N - i
+{
+  if i != N
+  then T2(N, i+1) + 1.0
+  else 0.0
+}
+
+lemma lem_fBigOlin() returns (c:R0, n0:nat)
+  ensures c > 0.0 && bigOfrom(c, n0, f, linGrowth())
+{
+  c, n0 := 1.0, 1;
+  forall n:nat | 0 <= n0 <= n
+    ensures f(n) <= c*linGrowth()(n)
+  {
+    calc {
+         f(n);
+      == n as R0;
+      == { lem_expOne(n as R0); }
+         exp(n as R0, 1.0);
+      <= c*exp(n as R0, 1.0); 
+      == c*linGrowth()(n);  
+    }
+  }
+}
+
+method FibTtest() {
+  ghost var t;
+  var r;
+  r, t := FibT(0); assert r == 0 && t == 0.0;
+  r, t := FibT(1); assert r == 1 && t == 1.0;
+  r, t := FibT(2); assert r == 1 && t == 2.0;
+  r, t := FibT(3); assert r == 2 && t == 3.0;
+  r, t := FibT(4); assert r == 3 && t == 4.0;
+  r, t := FibT(5); assert r == 5 && t == 5.0;
+  r, t := FibT(6); assert r == 8 && t == 6.0;
+}
